<?xml version="1.0"?>
<rdf:RDF xmlns="http://www.semanticweb.org/utente/ontologies/2024/9/CT_ontology/"
     xml:base="http://www.semanticweb.org/utente/ontologies/2024/9/CT_ontology/"
     xmlns:dc="http://purl.org/dc/elements/1.1/"
     xmlns:owl="http://www.w3.org/2002/07/owl#"
     xmlns:rdf="http://www.w3.org/1999/02/22-rdf-syntax-ns#"
     xmlns:xml="http://www.w3.org/XML/1998/namespace"
     xmlns:xsd="http://www.w3.org/2001/XMLSchema#"
     xmlns:rdfs="http://www.w3.org/2000/01/rdf-schema#"
     xmlns:schema="https://w3id.org/framester/schema/">
    <owl:Ontology rdf:about="http://www.semanticweb.org/utente/ontologies/2024/9/CT_ontology">
        <owl:imports rdf:resource="http://www.ontologydesignpatterns.org/ont/persp/perspectivisation.owl"/>
    </owl:Ontology>
    


    <!-- 
    ///////////////////////////////////////////////////////////////////////////////////////
    //
    // Object Properties
    //
    ///////////////////////////////////////////////////////////////////////////////////////
     -->

    


    <!-- http://www.semanticweb.org/utente/ontologies/2024/9/CT_ontology#InterpretedWith -->

    <owl:ObjectProperty rdf:about="http://www.semanticweb.org/utente/ontologies/2024/9/CT_ontology#InterpretedWith">
        <rdfs:domain rdf:resource="http://www.ontologydesignpatterns.org/ont/persp/perspectivisation.owl#Eventuality"/>
        <rdfs:range rdf:resource="http://www.ontologydesignpatterns.org/ont/persp/perspectivisation.owl#Cut"/>
    </owl:ObjectProperty>
    


    <!-- http://www.semanticweb.org/utente/ontologies/2024/9/CT_ontology#comesFrom -->

    <owl:ObjectProperty rdf:about="http://www.semanticweb.org/utente/ontologies/2024/9/CT_ontology#comesFrom">
        <rdfs:domain rdf:resource="http://www.ontologydesignpatterns.org/ont/persp/perspectivisation.owl#Eventuality"/>
        <rdfs:range rdf:resource="http://www.ontologydesignpatterns.org/ont/persp/perspectivisation.owl#Background"/>
    </owl:ObjectProperty>
    


    <!-- http://www.semanticweb.org/utente/ontologies/2024/9/CT_ontology#conveys -->

    <owl:ObjectProperty rdf:about="http://www.semanticweb.org/utente/ontologies/2024/9/CT_ontology#conveys">
        <rdfs:domain rdf:resource="http://www.ontologydesignpatterns.org/ont/persp/perspectivisation.owl#Cut"/>
        <rdfs:range rdf:resource="http://www.ontologydesignpatterns.org/ont/persp/perspectivisation.owl#Attitude"/>
    </owl:ObjectProperty>
    


    <!-- http://www.semanticweb.org/utente/ontologies/2024/9/CT_ontology#gives -->

    <owl:ObjectProperty rdf:about="http://www.semanticweb.org/utente/ontologies/2024/9/CT_ontology#gives">
        <rdfs:domain>
            <owl:Class>
                <owl:intersectionOf rdf:parseType="Collection">
                    <rdf:Description rdf:about="http://www.semanticweb.org/utente/ontologies/2024/9/CT_ontology#Expert"/>
                    <rdf:Description rdf:about="http://www.semanticweb.org/utente/ontologies/2024/9/CT_ontology#Scientist"/>
                    <rdf:Description rdf:about="http://www.semanticweb.org/utente/ontologies/2024/9/CT_ontology#Witness"/>
                </owl:intersectionOf>
            </owl:Class>
        </rdfs:domain>
        <rdfs:range rdf:resource="http://www.semanticweb.org/utente/ontologies/2024/9/CT_ontology#Testimony"/>
    </owl:ObjectProperty>
    


    <!-- http://www.semanticweb.org/utente/ontologies/2024/9/CT_ontology#hasComponent -->

    <owl:ObjectProperty rdf:about="http://www.semanticweb.org/utente/ontologies/2024/9/CT_ontology#hasComponent">
        <rdfs:range>
            <owl:Class>
                <owl:unionOf rdf:parseType="Collection">
                    <rdf:Description rdf:about="http://www.ontologydesignpatterns.org/ont/persp/perspectivisation.owl#Cut"/>
                    <rdf:Description rdf:about="http://www.ontologydesignpatterns.org/ont/persp/perspectivisation.owl#Eventuality"/>
                </owl:unionOf>
            </owl:Class>
        </rdfs:range>
    </owl:ObjectProperty>
    


    <!-- http://www.semanticweb.org/utente/ontologies/2024/9/CT_ontology#shotThrough -->

    <owl:ObjectProperty rdf:about="http://www.semanticweb.org/utente/ontologies/2024/9/CT_ontology#shotThrough">
        <rdfs:domain rdf:resource="http://www.ontologydesignpatterns.org/ont/persp/perspectivisation.owl#Cut"/>
        <rdfs:range rdf:resource="http://www.ontologydesignpatterns.org/ont/persp/perspectivisation.owl#Lens"/>
    </owl:ObjectProperty>
    


    <!-- http://www.semanticweb.org/utente/ontologies/2024/9/CT_ontology#viewedThrough -->

    <owl:ObjectProperty rdf:about="http://www.semanticweb.org/utente/ontologies/2024/9/CT_ontology#viewedThrough">
        <rdfs:domain rdf:resource="http://www.ontologydesignpatterns.org/ont/persp/perspectivisation.owl#Eventuality"/>
        <rdfs:range rdf:resource="http://www.ontologydesignpatterns.org/ont/persp/perspectivisation.owl#Lens"/>
    </owl:ObjectProperty>
    


    <!-- http://www.semanticweb.org/utente/ontologies/2024/9/CT_ontology#writes -->

    <owl:ObjectProperty rdf:about="http://www.semanticweb.org/utente/ontologies/2024/9/CT_ontology#writes">
        <rdfs:domain rdf:resource="http://www.semanticweb.org/utente/ontologies/2024/9/CT_ontology#Investigator"/>
        <rdfs:range rdf:resource="http://www.semanticweb.org/utente/ontologies/2024/9/CT_ontology#Report"/>
    </owl:ObjectProperty>
    


    <!-- 
    ///////////////////////////////////////////////////////////////////////////////////////
    //
    // Classes
    //
    ///////////////////////////////////////////////////////////////////////////////////////
     -->

    


    <!-- http://www.ontologydesignpatterns.org/cp/owl/agentrole.owl#Agent -->

    <owl:Class rdf:about="http://www.ontologydesignpatterns.org/cp/owl/agentrole.owl#Agent">
        <rdfs:subClassOf rdf:resource="http://www.ontologydesignpatterns.org/ont/persp/perspectivisation.owl#PerspectivisationTheorySituation"/>
        <rdfs:comment>The conceptualizer or perspective holder</rdfs:comment>
    </owl:Class>
    


    <!-- http://www.ontologydesignpatterns.org/ont/persp/perspectivisation.owl#Attitude -->

    <owl:Class rdf:about="http://www.ontologydesignpatterns.org/ont/persp/perspectivisation.owl#Attitude">
        <rdfs:comment>The attitude of a conceptualiser towards an eventuality, perspectivised through the application of a lens.</rdfs:comment>
    </owl:Class>
    


    <!-- http://www.ontologydesignpatterns.org/ont/persp/perspectivisation.owl#Background -->

    <owl:Class rdf:about="http://www.ontologydesignpatterns.org/ont/persp/perspectivisation.owl#Background">
        <rdfs:comment>The background knowledge for an eventuality targeted by perspectivisation.</rdfs:comment>
    </owl:Class>
    


    <!-- http://www.ontologydesignpatterns.org/ont/persp/perspectivisation.owl#Cut -->

    <owl:Class rdf:about="http://www.ontologydesignpatterns.org/ont/persp/perspectivisation.owl#Cut">
        <rdfs:comment>The cut emerging from perspectivising an eventuality through a lens.</rdfs:comment>
    </owl:Class>
    


    <!-- http://www.ontologydesignpatterns.org/ont/persp/perspectivisation.owl#Eventuality -->

    <owl:Class rdf:about="http://www.ontologydesignpatterns.org/ont/persp/perspectivisation.owl#Eventuality">
        <rdfs:comment>The eventuality targeted by perspectivisation, explicitly or implicitly extracted from its background knowledge.</rdfs:comment>
    </owl:Class>
    


    <!-- http://www.ontologydesignpatterns.org/ont/persp/perspectivisation.owl#Lens -->

    <owl:Class rdf:about="http://www.ontologydesignpatterns.org/ont/persp/perspectivisation.owl#Lens">
        <rdfs:comment>The lens used by perspectivisation on an eventuality.</rdfs:comment>
    </owl:Class>
    


    <!-- http://www.semanticweb.org/utente/ontologies/2024/9/CT_ontology#AdvocancyCut -->

    <owl:Class rdf:about="http://www.semanticweb.org/utente/ontologies/2024/9/CT_ontology#AdvocancyCut">
        <rdfs:subClassOf rdf:resource="http://www.ontologydesignpatterns.org/ont/persp/perspectivisation.owl#Cut"/>
        <rdfs:comment>Represents interpretations that actively support and advocate for the conspiracy theory.</rdfs:comment>
    </owl:Class>
    


    <!-- http://www.semanticweb.org/utente/ontologies/2024/9/CT_ontology#Community -->

    <owl:Class rdf:about="http://www.semanticweb.org/utente/ontologies/2024/9/CT_ontology#Community">
        <rdfs:subClassOf rdf:resource="http://www.ontologydesignpatterns.org/cp/owl/agentrole.owl#Agent"/>
        <owl:disjointWith rdf:resource="http://www.semanticweb.org/utente/ontologies/2024/9/CT_ontology#Person"/>
        <rdfs:comment>Any group of people who share the same goal</rdfs:comment>
    </owl:Class>
    


    <!-- http://www.semanticweb.org/utente/ontologies/2024/9/CT_ontology#CompromisingCut -->

    <owl:Class rdf:about="http://www.semanticweb.org/utente/ontologies/2024/9/CT_ontology#CompromisingCut">
        <rdfs:subClassOf rdf:resource="http://www.ontologydesignpatterns.org/ont/persp/perspectivisation.owl#Cut"/>
        <rdfs:comment>Represents perspectives or interpretations that expose weaknesses or flaws in a conspiracy theory.</rdfs:comment>
    </owl:Class>
    


    <!-- http://www.semanticweb.org/utente/ontologies/2024/9/CT_ontology#ConspiracyLens -->

    <owl:Class rdf:about="http://www.semanticweb.org/utente/ontologies/2024/9/CT_ontology#ConspiracyLens">
        <rdfs:subClassOf rdf:resource="http://www.ontologydesignpatterns.org/ont/persp/perspectivisation.owl#Lens"/>
        <rdfs:comment>The lens used by a conspiracy theory group or individual. Supports a conspiracy.</rdfs:comment>
    </owl:Class>
    


    <!-- http://www.semanticweb.org/utente/ontologies/2024/9/CT_ontology#ConspiracyTheoryGroup -->

    <owl:Class rdf:about="http://www.semanticweb.org/utente/ontologies/2024/9/CT_ontology#ConspiracyTheoryGroup">
        <rdfs:subClassOf rdf:resource="http://www.semanticweb.org/utente/ontologies/2024/9/CT_ontology#Community"/>
        <rdfs:comment>Any group of individuals who share the same support for a conspiracy theory, usually with the same talking points.</rdfs:comment>
    </owl:Class>
    


    <!-- http://www.semanticweb.org/utente/ontologies/2024/9/CT_ontology#EmotionalCut -->

    <owl:Class rdf:about="http://www.semanticweb.org/utente/ontologies/2024/9/CT_ontology#EmotionalCut">
        <rdfs:subClassOf rdf:resource="http://www.ontologydesignpatterns.org/ont/persp/perspectivisation.owl#Cut"/>
        <rdfs:comment>Represents interpretations driven by emotional appeals.</rdfs:comment>
    </owl:Class>
    


    <!-- http://www.semanticweb.org/utente/ontologies/2024/9/CT_ontology#Expert -->

    <owl:Class rdf:about="http://www.semanticweb.org/utente/ontologies/2024/9/CT_ontology#Expert">
        <rdfs:subClassOf rdf:resource="http://www.semanticweb.org/utente/ontologies/2024/9/CT_ontology#Person"/>
        <rdfs:comment>An individual highly specialized in a topic or discipline.</rdfs:comment>
    </owl:Class>
    


    <!-- http://www.semanticweb.org/utente/ontologies/2024/9/CT_ontology#GeneralPublic -->

    <owl:Class rdf:about="http://www.semanticweb.org/utente/ontologies/2024/9/CT_ontology#GeneralPublic">
        <rdfs:subClassOf rdf:resource="http://www.semanticweb.org/utente/ontologies/2024/9/CT_ontology#Community"/>
        <rdfs:comment>All or most people, especially those not part of a specified group; ordinary people as opposed to officials, experts, politicians, conspiracists...</rdfs:comment>
    </owl:Class>
    


    <!-- http://www.semanticweb.org/utente/ontologies/2024/9/CT_ontology#Government -->

    <owl:Class rdf:about="http://www.semanticweb.org/utente/ontologies/2024/9/CT_ontology#Government">
        <rdfs:subClassOf rdf:resource="http://www.semanticweb.org/utente/ontologies/2024/9/CT_ontology#Community"/>
        <rdfs:comment>The group of people with the authority to govern a country or state.</rdfs:comment>
    </owl:Class>
    


    <!-- http://www.semanticweb.org/utente/ontologies/2024/9/CT_ontology#GovernmentLens -->

    <owl:Class rdf:about="http://www.semanticweb.org/utente/ontologies/2024/9/CT_ontology#GovernmentLens">
        <rdfs:subClassOf rdf:resource="http://www.ontologydesignpatterns.org/ont/persp/perspectivisation.owl#Lens"/>
        <rdfs:comment>The lens used by the govenment, produces the official narrative.</rdfs:comment>
    </owl:Class>
    


    <!-- http://www.semanticweb.org/utente/ontologies/2024/9/CT_ontology#HistoricalContext -->

    <owl:Class rdf:about="http://www.semanticweb.org/utente/ontologies/2024/9/CT_ontology#HistoricalContext">
        <rdfs:subClassOf rdf:resource="http://www.ontologydesignpatterns.org/ont/persp/perspectivisation.owl#Background"/>
        <owl:disjointWith rdf:resource="http://www.semanticweb.org/utente/ontologies/2024/9/CT_ontology#PersonalExperience"/>
        <rdfs:comment>The ensemble of historical knowledge, usually (but not always) learned or taught in school.</rdfs:comment>
    </owl:Class>
    


    <!-- http://www.semanticweb.org/utente/ontologies/2024/9/CT_ontology#Investigator -->

    <owl:Class rdf:about="http://www.semanticweb.org/utente/ontologies/2024/9/CT_ontology#Investigator">
        <rdfs:subClassOf rdf:resource="http://www.semanticweb.org/utente/ontologies/2024/9/CT_ontology#Person"/>
        <rdfs:comment>Individual who finds the proofs supporting a conspiracy theory.</rdfs:comment>
    </owl:Class>
    


    <!-- http://www.semanticweb.org/utente/ontologies/2024/9/CT_ontology#MediaLens -->

    <owl:Class rdf:about="http://www.semanticweb.org/utente/ontologies/2024/9/CT_ontology#MediaLens">
        <rdfs:subClassOf rdf:resource="http://www.ontologydesignpatterns.org/ont/persp/perspectivisation.owl#Lens"/>
        <rdfs:comment>The lens used by media outlets.</rdfs:comment>
    </owl:Class>
    


    <!-- http://www.semanticweb.org/utente/ontologies/2024/9/CT_ontology#Object -->

    <owl:Class rdf:about="http://www.semanticweb.org/utente/ontologies/2024/9/CT_ontology#Object">
        <rdfs:subClassOf rdf:resource="http://www.ontologydesignpatterns.org/ont/persp/perspectivisation.owl#Eventuality"/>
        <rdfs:comment>Could be a document, a video or any material thing that could be interpreted with a cut.</rdfs:comment>
    </owl:Class>
    


    <!-- http://www.semanticweb.org/utente/ontologies/2024/9/CT_ontology#Person -->

    <owl:Class rdf:about="http://www.semanticweb.org/utente/ontologies/2024/9/CT_ontology#Person">
        <rdfs:subClassOf rdf:resource="http://www.ontologydesignpatterns.org/cp/owl/agentrole.owl#Agent"/>
        <rdfs:comment>A singular individual</rdfs:comment>
    </owl:Class>
    


    <!-- http://www.semanticweb.org/utente/ontologies/2024/9/CT_ontology#PersonalExperience -->

    <owl:Class rdf:about="http://www.semanticweb.org/utente/ontologies/2024/9/CT_ontology#PersonalExperience">
        <rdfs:subClassOf rdf:resource="http://www.ontologydesignpatterns.org/ont/persp/perspectivisation.owl#Background"/>
        <rdfs:comment>The knowledge gained through life, often by chance, as opposed to the knowledge taught in school, which is instead usually planned and common between individuals.</rdfs:comment>
    </owl:Class>
    


    <!-- http://www.semanticweb.org/utente/ontologies/2024/9/CT_ontology#Report -->

    <owl:Class rdf:about="http://www.semanticweb.org/utente/ontologies/2024/9/CT_ontology#Report">
        <rdfs:subClassOf rdf:resource="http://www.ontologydesignpatterns.org/ont/persp/perspectivisation.owl#Eventuality"/>
        <rdfs:comment>A written account given of a particular matter, especially in the form of an official document, after thorough investigation by a person or body.</rdfs:comment>
    </owl:Class>
    


    <!-- http://www.semanticweb.org/utente/ontologies/2024/9/CT_ontology#ScienceLens -->

    <owl:Class rdf:about="http://www.semanticweb.org/utente/ontologies/2024/9/CT_ontology#ScienceLens">
        <rdfs:subClassOf rdf:resource="http://www.ontologydesignpatterns.org/ont/persp/perspectivisation.owl#Lens"/>
        <rdfs:comment>The lens used by the scientific community or by an individual scientist. Usually does not support a conspiracy theory.</rdfs:comment>
    </owl:Class>
    


    <!-- http://www.semanticweb.org/utente/ontologies/2024/9/CT_ontology#ScientificCommunity -->

    <owl:Class rdf:about="http://www.semanticweb.org/utente/ontologies/2024/9/CT_ontology#ScientificCommunity">
        <rdfs:subClassOf rdf:resource="http://www.semanticweb.org/utente/ontologies/2024/9/CT_ontology#Community"/>
        <rdfs:comment>The community of all the scientists who usually homogeneously share similar opinions and conclusions towards conspiracy theories.</rdfs:comment>
    </owl:Class>
    


    <!-- http://www.semanticweb.org/utente/ontologies/2024/9/CT_ontology#Scientist -->

    <owl:Class rdf:about="http://www.semanticweb.org/utente/ontologies/2024/9/CT_ontology#Scientist">
        <rdfs:subClassOf rdf:resource="http://www.semanticweb.org/utente/ontologies/2024/9/CT_ontology#Person"/>
        <rdfs:comment>Member of the scientific community, must be a scientist.</rdfs:comment>
    </owl:Class>
    


    <!-- http://www.semanticweb.org/utente/ontologies/2024/9/CT_ontology#Testimony -->

    <owl:Class rdf:about="http://www.semanticweb.org/utente/ontologies/2024/9/CT_ontology#Testimony">
        <rdfs:subClassOf rdf:resource="http://www.ontologydesignpatterns.org/ont/persp/perspectivisation.owl#Eventuality"/>
        <rdfs:comment>A formal written of spoken statement, a recalling of a personally-experienced event.</rdfs:comment>
    </owl:Class>
    


    <!-- http://www.semanticweb.org/utente/ontologies/2024/9/CT_ontology#Whistleblower -->

    <owl:Class rdf:about="http://www.semanticweb.org/utente/ontologies/2024/9/CT_ontology#Whistleblower">
        <rdfs:subClassOf rdf:resource="http://www.semanticweb.org/utente/ontologies/2024/9/CT_ontology#Person"/>
        <rdfs:comment>Insider of a community accused of nefarious actions by the conspiracy theory who reveals important information regarding the wrongdoings of said community.</rdfs:comment>
    </owl:Class>
    


    <!-- http://www.semanticweb.org/utente/ontologies/2024/9/CT_ontology#Witness -->

    <owl:Class rdf:about="http://www.semanticweb.org/utente/ontologies/2024/9/CT_ontology#Witness">
        <rdfs:subClassOf rdf:resource="http://www.semanticweb.org/utente/ontologies/2024/9/CT_ontology#Person"/>
        <rdfs:comment>Individual who offers their testimony.</rdfs:comment>
    </owl:Class>
    


    <!-- http://www.semanticweb.org/utente/ontologies/2024/CT_ontology#Event -->

    <owl:Class rdf:about="http://www.semanticweb.org/utente/ontologies/2024/CT_ontology#Event">
        <rdfs:subClassOf rdf:resource="http://www.ontologydesignpatterns.org/ont/persp/perspectivisation.owl#Eventuality"/>
        <rdfs:comment>A thing that happens or takes place, especially one of importance.</rdfs:comment>
    </owl:Class>
    


    <!-- 
    ///////////////////////////////////////////////////////////////////////////////////////
    //
    // Individuals
    //
    ///////////////////////////////////////////////////////////////////////////////////////
     -->

    


    <!-- http://www.semanticweb.org/utente/ontologies/2024/9/CT_ontology#NegativeAttitude -->

    <owl:NamedIndividual rdf:about="http://www.semanticweb.org/utente/ontologies/2024/9/CT_ontology#NegativeAttitude">
        <rdf:type rdf:resource="http://www.ontologydesignpatterns.org/ont/persp/perspectivisation.owl#Attitude"/>
        <rdfs:comment>Any type of attitude which interprets negatively an eventuality, meaning that produces a not favourable cut towards an eventuality.</rdfs:comment>
    </owl:NamedIndividual>
    


    <!-- http://www.semanticweb.org/utente/ontologies/2024/9/CT_ontology#NeutralAttitude -->

    <owl:NamedIndividual rdf:about="http://www.semanticweb.org/utente/ontologies/2024/9/CT_ontology#NeutralAttitude">
        <rdf:type rdf:resource="http://www.ontologydesignpatterns.org/ont/persp/perspectivisation.owl#Attitude"/>
        <rdfs:comment>Any type of attitude which interprets neutrally an eventuality, meaning that produces an unbiased cut towards an eventuality.</rdfs:comment>
    </owl:NamedIndividual>
    


    <!-- http://www.semanticweb.org/utente/ontologies/2024/9/CT_ontology#PositiveAttitude -->

    <owl:NamedIndividual rdf:about="http://www.semanticweb.org/utente/ontologies/2024/9/CT_ontology#PositiveAttitude">
        <rdf:type rdf:resource="http://www.ontologydesignpatterns.org/ont/persp/perspectivisation.owl#Attitude"/>
        <rdfs:comment>Any type of attitude which interprets positively an eventuality, meaning that produces a  favourable cut towards an eventuality.</rdfs:comment>
    </owl:NamedIndividual>
    


    <!-- http://www.semanticweb.org/utente/ontologies/2024/9/CT_ontology#ProponentAttitude -->

    <owl:NamedIndividual rdf:about="http://www.semanticweb.org/utente/ontologies/2024/9/CT_ontology#ProponentAttitude">
        <rdf:type rdf:resource="http://www.ontologydesignpatterns.org/ont/persp/perspectivisation.owl#Attitude"/>
        <rdfs:comment>Any type of attitude which interprets an eventuality as a supporting element towards a conspiracy theory.</rdfs:comment>
    </owl:NamedIndividual>
    


    <!-- http://www.semanticweb.org/utente/ontologies/2024/9/CT_ontology#SkepticalAttitude -->

    <owl:NamedIndividual rdf:about="http://www.semanticweb.org/utente/ontologies/2024/9/CT_ontology#SkepticalAttitude">
        <rdf:type rdf:resource="http://www.ontologydesignpatterns.org/ont/persp/perspectivisation.owl#Attitude"/>
        <rdfs:comment>Any type of attitude which interprets an eventuality as a contrasting element against a conspiracy theory.</rdfs:comment>
    </owl:NamedIndividual>
    


    <!-- 
    ///////////////////////////////////////////////////////////////////////////////////////
    //
    // General axioms
    //
    ///////////////////////////////////////////////////////////////////////////////////////
     -->

    <rdf:Description>
        <rdf:type rdf:resource="http://www.w3.org/2002/07/owl#AllDisjointClasses"/>
        <owl:members rdf:parseType="Collection">
            <rdf:Description rdf:about="http://www.ontologydesignpatterns.org/cp/owl/agentrole.owl#Agent"/>
            <rdf:Description rdf:about="http://www.ontologydesignpatterns.org/ont/persp/perspectivisation.owl#Attitude"/>
            <rdf:Description rdf:about="http://www.ontologydesignpatterns.org/ont/persp/perspectivisation.owl#Background"/>
            <rdf:Description rdf:about="http://www.ontologydesignpatterns.org/ont/persp/perspectivisation.owl#Cut"/>
            <rdf:Description rdf:about="http://www.ontologydesignpatterns.org/ont/persp/perspectivisation.owl#Eventuality"/>
            <rdf:Description rdf:about="http://www.ontologydesignpatterns.org/ont/persp/perspectivisation.owl#Lens"/>
        </owl:members>
    </rdf:Description>
    <rdf:Description>
        <rdf:type rdf:resource="http://www.w3.org/2002/07/owl#AllDisjointClasses"/>
        <owl:members rdf:parseType="Collection">
            <rdf:Description rdf:about="http://www.semanticweb.org/utente/ontologies/2024/9/CT_ontology#AdvocancyCut"/>
            <rdf:Description rdf:about="http://www.semanticweb.org/utente/ontologies/2024/9/CT_ontology#CompromisingCut"/>
            <rdf:Description rdf:about="http://www.semanticweb.org/utente/ontologies/2024/9/CT_ontology#EmotionalCut"/>
        </owl:members>
    </rdf:Description>
    <rdf:Description>
        <rdf:type rdf:resource="http://www.w3.org/2002/07/owl#AllDisjointClasses"/>
        <owl:members rdf:parseType="Collection">
            <rdf:Description rdf:about="http://www.semanticweb.org/utente/ontologies/2024/9/CT_ontology#ConspiracyLens"/>
            <rdf:Description rdf:about="http://www.semanticweb.org/utente/ontologies/2024/9/CT_ontology#GovernmentLens"/>
            <rdf:Description rdf:about="http://www.semanticweb.org/utente/ontologies/2024/9/CT_ontology#MediaLens"/>
            <rdf:Description rdf:about="http://www.semanticweb.org/utente/ontologies/2024/9/CT_ontology#ScienceLens"/>
        </owl:members>
    </rdf:Description>
    <rdf:Description>
        <rdf:type rdf:resource="http://www.w3.org/2002/07/owl#AllDisjointClasses"/>
        <owl:members rdf:parseType="Collection">
            <rdf:Description rdf:about="http://www.semanticweb.org/utente/ontologies/2024/9/CT_ontology#ConspiracyTheoryGroup"/>
            <rdf:Description rdf:about="http://www.semanticweb.org/utente/ontologies/2024/9/CT_ontology#GeneralPublic"/>
            <rdf:Description rdf:about="http://www.semanticweb.org/utente/ontologies/2024/9/CT_ontology#Government"/>
            <rdf:Description rdf:about="http://www.semanticweb.org/utente/ontologies/2024/9/CT_ontology#ScientificCommunity"/>
        </owl:members>
    </rdf:Description>
    <rdf:Description>
        <rdf:type rdf:resource="http://www.w3.org/2002/07/owl#AllDisjointClasses"/>
        <owl:members rdf:parseType="Collection">
            <rdf:Description rdf:about="http://www.semanticweb.org/utente/ontologies/2024/9/CT_ontology#Object"/>
            <rdf:Description rdf:about="http://www.semanticweb.org/utente/ontologies/2024/9/CT_ontology#Report"/>
            <rdf:Description rdf:about="http://www.semanticweb.org/utente/ontologies/2024/9/CT_ontology#Testimony"/>
            <rdf:Description rdf:about="http://www.semanticweb.org/utente/ontologies/2024/CT_ontology#Event"/>
        </owl:members>
    </rdf:Description>
</rdf:RDF>



<!-- Generated by the OWL API (version 4.5.26.2023-07-17T20:34:13Z) https://github.com/owlcs/owlapi -->

